Remove _composite_state and _composite_label indirection
This removes the indirection of defining the actual composite state
and label types as _composite_state and _composite_label and making
the nice names composite_state and composite_label definitions that
expand to field projections from the VLSMType composite_type.
This helped typechecking unify (composite_state ?IM) against
some (@state _ ?vtype), without needing to know the expected VLSMType.
The need for this indirection was removed by declaring composite_type
a Canonical Structure, so typechecking will try the guess that vtype
should be some (composite_state _) when otherwise stuck on a
unification problem like that, and also by giving VLSMMachine a
"bidirectionality hint" so typechecking record expressions of
VLSMMachines like composite_vlsm_machine will consider the expected
result type (explicitly given as VLSMMachine composite_type) rather
than needing to discover a vtype by unification at all.

theories/VLSM/Core/Composition.v
@@ -39,7 +39,7 @@ machine <<n>>.
 Note that the [composite_state] type is the dependent product type of the
 family of [state] types corresponding to each index.
 *)
-    Definition _composite_state : Type :=
+    Definition composite_state : Type :=
       forall n : index, vstate (IM n).
 
 (**
@@ -48,17 +48,15 @@ A [composite_label] is a pair between an index <<N>> and a [label] of <<IT n>>.
 Note that the [composite_label] type is the dependent sum of the family of
 types <<[@label _ (IT n) | n <- index]>>.
 *)
-    Definition _composite_label
+    Definition composite_label
       : Type
       := sigT (fun n => vlabel (IM n)).
 
-    Definition composite_type : VLSMType message :=
-      {| state := _composite_state
-       ; label := _composite_label
+    Canonical Structure composite_type : VLSMType message :=
+      {| state := composite_state
+       ; label := composite_label
       |}.
 
-    Definition composite_state := @state message composite_type.
-    Definition composite_label := @label message composite_type.
     Definition composite_transition_item : Type := @transition_item message composite_type.
 
 (**
@@ -310,10 +308,10 @@ the [composite_valid]ity.
       (constraint : composite_label -> composite_state * option message -> Prop)
       : VLSMMachine composite_type
       :=
-      {|  initial_state_prop := composite_initial_state_prop
-       ;  initial_message_prop := composite_initial_message_prop
-       ;  transition := composite_transition
-       ;  valid := constrained_composite_valid constraint
+      {| initial_state_prop := composite_initial_state_prop
+       ; initial_message_prop := composite_initial_message_prop
+       ; transition := composite_transition
+       ; valid := constrained_composite_valid constraint
       |}.
 
     Definition composite_vlsm
@@ -832,7 +830,7 @@ Qed.
 
 Lemma composite_transition_project_active
       message `{EqDecision index} (IM : index -> VLSM message)
-  : forall (l : label) (s : state) (im : option message) (s' : state) (om : option message),
+  : forall (l : composite_label IM) (s : composite_state IM) (im : option message) (s' : composite_state IM) (om : option message),
       composite_transition IM l (s, im) = (s', om) ->
       vtransition (IM (projT1 l)) (projT2 l) (s (projT1 l), im) = (s' (projT1 l), om).
 Proof.
